coq/TypedParsing.v
@@ -47,21 +47,7 @@ Definition function
   {sig tau} :=
     Types.InternalFunction' fn_name_t
       (TypedSyntax.action pos_t var_t fn_name_t R Sigma sig tau).
-(*
 
-TODO example
-
-reg1 : bits_t 4
-reg2 : btis_t 5
-
-
-0b"001100110" && (read(reg1) ++ read(reg2))
-
-bits_t 9 -> concat also has to be bits_t 9
-
-but has type ?a + ?b -> need bidirectionaly but not possible here
-
-*)
 (* When checking a concatenation we need to use the
  * bidirectionality hint before the arguments. Thats
  * because we need the unification to resolve R and Sigma
@@ -90,21 +76,14 @@ Local Definition delay_tau_uni {reg_t ext_fn_t}
     match proof with
     | eq_refl => a
     end.
-Arguments delay_tau_uni {reg_t ext_fn_t} {R Sigma} {sig tau_in tau_out} & a proof : assert.
+Arguments delay_tau_uni & {reg_t ext_fn_t} {R Sigma} {sig tau_in tau_out} a proof : assert.
 Notation delay_tau a := (delay_tau_uni a eq_refl).
-
-(* Local Definition proof_mem_eq {K} {sig} {k1 k2 : K} (m : member k1 sig) (proof : k1 = k2) : member k2 sig :=
-    match proof with
-    | eq_refl => m
-    end.
-Arguments proof_mem_eq {K} {sig} {k1 k2} m & proof : assert.
-Notation mem_eq m := (proof_mem_eq m eq_refl). *)
 
 Declare Custom Entry koika_t.
 
 (* This is the entry point to transition from normal
   coq (constr) to koika *)
-Notation "'<{' e '}>'" := ltac:(e) (e custom koika_t).
+Notation "'<{' e '}>'" := (e) (e custom koika_t).
 
 (* Koika_var *)
 Declare Custom Entry koika_t_var.
@@ -114,21 +93,6 @@ Notation "a" := (a) (in custom koika_t_var at level 0, a ident, format "'[' a ']
 
 (* TODO better error messages *)
 (* TODO explain why this class is necessary in the first place *)
-
-
-(* Definition var_ref_opt (k: var_t) sig : member (k, match assoc k sig with
-| Some a => a.1
-| None => unit_t
-end) sig :=
-  match assoc k sig as e return
-    match e with
-    | Some a => member (k, a.1) sig
-    | None => unit_t
-    end
-  with
-  | Some a => a.2
-  | None => Ob
-  end. *)
 
 
 (* Variable references
@@ -169,39 +133,39 @@ end) sig :=
  * no typclass instance could be constructed and type checking
  * fails)
  *)
-(* Inductive member2 {K: Type}: list K -> K -> Type :=
-| Member2Hd: forall k sig, member2 (k :: sig) k
-| Member2Tl: forall k k' sig, member2 sig k -> member2 (k' :: sig) k. *)
 
 (* since typeclasses are only resolved after the normal type checking is done
   the value of `tau` is not known during type checking - however some places need
   to know the precise value of the variable, for that this new type more precise
   type makes sure that the tau
 *)
-Definition get_type (k: var_t) sig : type :=
+Definition var_type (k: var_t) sig : type :=
   match assoc k sig with
   | Some a => a.1
   | None => unit_t
   end.
 
-Class VarRef (k: var_t) sig := var_ref : member (k, get_type k sig) sig.
+Class VarRef (k: var_t) sig := var_ref : member (k, var_type k sig) sig.
 Hint Mode VarRef + + : typeclass_instances.
 Arguments var_ref k & sig {VarRef} : assert.
 Hint Extern 1 (VarRef ?k ?sig) => exact (projT2 (must (assoc k sig))) : typeclass_instances.
 
-(* Get the instance out of an optional
- *)
-(* Class MustClass {A} (o : option A) := must_class : A.
-Hint Mode MustClass + + : typeclass_instances.
-Arguments must_class {A} o {MustClass} : assert.
-Hint Extern 1 (MustClass ?o) => exact (must o) : typeclass_instances. *)
-
 (* Koika_types *)
 (* TODO improve arg list to be more consistent on nil case  *)
 Declare Custom Entry koika_t_binder.
-Notation "'(' x ':' y ')'" := (x%string, (y : type)) (in custom koika_t_binder at level 0, x custom koika_t_var, y constr).
-Notation "a  ..  b" := (cons a ..  (cons b nil) ..)  (in custom koika_t_binder at level 1, a custom koika_t_binder at next level, b custom koika_t_binder at next level).
+(* Notation "'(' x ':' y ')'" := [(x%string, (y : type))] (in custom koika_t_binder at level 0, x custom koika_t_var, y constr). *)
+(* Max: I dislike this style as it contrasts with the style of coq.
+    In my opinion the syntax should be at least consistent.
+    Either like in C: (a1 : type, a2 : type, ...) and () for empty
+    Or like in Coq: (a1 a2 : type) (a3 : type) and literally nothing for empty
 
+    I dislike the current version which is mixing both
+*)
+Notation "x1 .. xn ':' y" := (cons (x1%string, (y : type)) .. (cons (xn%string, (y : type)) nil) .. ) (in custom koika_t_binder at level 0, x1 custom koika_t_var, xn custom koika_t_var, y constr).
+Notation "'(' a ')' b" := (app a b) (in custom koika_t_binder at level 1, a at next level, right associativity).
+Notation "'(' a ')'"   := a         (in custom koika_t_binder at level 1, a at next level).
+Notation "'(' ')'"     := nil       (in custom koika_t_binder at level 1).
+Notation "'()'"        := nil       (in custom koika_t_binder at level 1).
 
 (* We want to tell the typechecker that the body of the function
  * should have the function's arguments in its context (sig).
@@ -224,68 +188,70 @@ Notation "a  ..  b" := (cons a ..  (cons b nil) ..)  (in custom koika_t_binder a
 Arguments refine_sig_tau sig tau {reg_t ext_fn_t} {R Sigma} & a : assert. *)
 
 (* TODO prevent unfolding of functions on simpl/cbn - Arguments : simpl never ??*)
+(* TODO function without return type?  *)
+(* todo maybe wrap into delay_function_tau? *)
 Notation "'fun' nm args ':' ret '=>' body" :=
-  (@Build_InternalFunction' string (action' _ _ (tau := ret) (sig := args)) nm (delay_tau body))
+  (@Build_InternalFunction' string (action' _ _ (tau := ret) (sig := args)) nm body)
     (in custom koika_t at level 200, nm custom koika_t_var, args custom koika_t_binder, ret constr at level 0, right associativity, format "'[v' 'fun'  nm  args  ':'  ret  '=>' '/' body ']'").
-Notation "'fun' nm '()' ':' ret '=>' body" :=
-  (@Build_InternalFunction' string (action' _ _ (tau := ret) (sig := nil)) nm (delay_tau  body))
-    (in custom koika_t at level 200, nm custom koika_t_var, ret constr at level 0, right associativity, format "'[v' 'fun'  nm  '()'   ':'  ret  '=>' '/' body ']'").
+Notation "'fun' nm ':' ret '=>' body" :=
+  (@Build_InternalFunction' string (action' _ _ (tau := ret) (sig := nil)) nm body)
+    (in custom koika_t at level 200, nm custom koika_t_var, ret constr at level 0, right associativity, format "'[v' 'fun'  nm   ':'  ret  '=>' '/' body ']'").
 
-Notation "'assert' a 'in' c"          := (If (delay_tau a) c (Const (tau := unit_t) Ob)) (in custom koika_t at level 200, right associativity, format "'[v' 'assert'  a '/' 'in'  c ']'").
-Notation "'assert' a 'else' b 'in' c" := (If (delay_tau a) c (delay_tau b         )) (in custom koika_t at level 200, right associativity, format "'[v' 'assert'  a '/' 'else'  b '/' 'in'  c ']'").
-Notation "'when' a 'do' t "           := (If (delay_tau a) t (Const (tau := unit_t) Ob)) (in custom koika_t at level 200, right associativity, format "'[v' 'when'  a '/' 'do'  t '/' ']'").
+Notation "'assert' a 'in' c"          := (delay_tau (If a c (Const (tau := unit_t) Ob))) (in custom koika_t at level 200, right associativity, format "'[v' 'assert'  a '/' 'in'  c ']'").
+Notation "'assert' a 'else' b 'in' c" := (delay_tau (If a c b                         )) (in custom koika_t at level 200, right associativity, format "'[v' 'assert'  a '/' 'else'  b '/' 'in'  c ']'").
+Notation "'when' a 'do' t "           := (delay_tau (If a t (Const (tau := unit_t) Ob))) (in custom koika_t at level 200, right associativity, format "'[v' 'when'  a '/' 'do'  t '/' ']'").
 
-Notation "'let' a ':=' b 'in' c" := (Bind a b c) (in custom koika_t at level 200, a custom koika_t_var, right associativity, format "'[v' 'let'  a  ':='  b  'in' '/' c ']'").
-Notation "'let' a ':' typ ':=' b 'in' c" := (Bind (tau := typ) a b c) (in custom koika_t at level 200,
+Notation "'let' a ':=' b 'in' c" := (delay_tau (Bind a b c)) (in custom koika_t at level 200, a custom koika_t_var, right associativity, format "'[v' 'let'  a  ':='  b  'in' '/' c ']'").
+Notation "'let' a ':' typ ':=' b 'in' c" := (delay_tau (Bind (tau := typ) a b c)) (in custom koika_t at level 200,
   a custom koika_t_var,
   typ constr at level 0, right associativity, format "'[v' 'let'  a  ':' typ ':='  b  'in' '/' c ']'").
 
-Notation "a ';' b" := (Seq (delay_tau a)                          b) (in custom koika_t at level 90, b at level 200, format "'[v' a ';' '/' b ']'" ).
-Notation "a ';'"   := (Seq (delay_tau a) (Const (tau := unit_t) Ob)) (in custom koika_t at level 90). (* trailing comma *)
+Notation "a ';' b" := (delay_tau (Seq a                          b)) (in custom koika_t at level 90, b at level 200, format "'[v' a ';' '/' b ']'" ).
+Notation "a ';'"   := (delay_tau (Seq a (Const (tau := unit_t) Ob))) (in custom koika_t at level 90). (* trailing comma *)
 
-Notation "'set' a ':=' b" := (Assign (var_ref a _) (delay_tau b)) (in custom koika_t at level 89, a custom koika_t_var, only parsing).
+Notation "'set' a ':=' b" := (delay_tau (Assign (var_ref a _) b)) (in custom koika_t at level 89, a custom koika_t_var, only parsing).
 
-Notation "'if' a 'then' t"            := (If (delay_tau a) t             (Const (tau := unit_t) Ob)) (in custom koika_t at level 89, t custom koika_t at level 89, right associativity, format "'[v' if  a '/' then  t ']'").
-Notation "'if' a 'then' t 'else' f"   := (If (delay_tau a) t                          (delay_tau f)) (in custom koika_t at level 89, t custom koika_t at level 89, right associativity, format "'[v' if  a '/' then  t '/' else  f ']'").
-Notation "'guard' '(' a ')' "         := (If (delay_tau a) (Const (tau := unit_t) Ob) (Fail unit_t)) (in custom koika_t at level 89, right associativity, format "'guard' '(' a ')'").
+Notation "'if' a 'then' t"            := (delay_tau (If a t             (Const (tau := unit_t) Ob))) (in custom koika_t at level 89, t custom koika_t at level 89, right associativity, format "'[v' if  a '/' then  t ']'").
+Notation "'if' a 'then' t 'else' f"   := (delay_tau (If a t                                     f )) (in custom koika_t at level 89, t custom koika_t at level 89, right associativity, format "'[v' if  a '/' then  t '/' else  f ']'").
+Notation "'guard' '(' a ')' "         := (delay_tau (If a (Const (tau := unit_t) Ob) (Fail unit_t))) (in custom koika_t at level 89, right associativity, format "'guard' '(' a ')'").
 
 (* Inspired by cpp the precedence  *)
 (* https://en.cppreference.com/w/cpp/language/operator_precedence *)
 (* TODO id really prefer to use || and && for logical operations and & | for bitwise *)
 (* Bit operations *)
-Notation "a  '||'  b"  := (Binop (Bits2 (Or       _))          (delay_tau a) (delay_tau b)) (in custom koika_t at level 85).
-Notation "a  '^'  b"   := (Binop (Bits2 (Xor      _))          (delay_tau a) (delay_tau b)) (in custom koika_t at level 84).
-Notation "a  '&&'  b"  := (Binop (Bits2 (And      _))          (delay_tau a) (delay_tau b)) (in custom koika_t at level 83).
+Notation "a  '||'  b"  := (delay_tau (Binop (Bits2 (Or       _))          a b)) (in custom koika_t at level 85).
+Notation "a  '^'  b"   := (delay_tau (Binop (Bits2 (Xor      _))          a b)) (in custom koika_t at level 84).
+Notation "a  '&&'  b"  := (delay_tau (Binop (Bits2 (And      _))          a b)) (in custom koika_t at level 83).
 
 (* Comparisons *)
-Notation "a  '!='  b"  := (Binop (Eq _ true)                   (delay_tau a) (delay_tau b)) (in custom koika_t at level 80).
-Notation "a  '=='  b"  := (Binop (Eq _ false)                  (delay_tau a) (delay_tau b)) (in custom koika_t at level 80).
+Notation "a  '!='  b"  := (delay_tau (Binop (Eq _ true)                   a b)) (in custom koika_t at level 80).
+Notation "a  '=='  b"  := (delay_tau (Binop (Eq _ false)                  a b)) (in custom koika_t at level 80).
 
-Notation "a  '<'  b"   := (Binop (Bits2 (Compare false cLt _)) (delay_tau a) (delay_tau b)) (in custom koika_t at level 79).
-Notation "a  '<s'  b"  := (Binop (Bits2 (Compare true  cLt _)) (delay_tau a) (delay_tau b)) (in custom koika_t at level 79).
-Notation "a  '<='  b"  := (Binop (Bits2 (Compare false cLe _)) (delay_tau a) (delay_tau b)) (in custom koika_t at level 79).
-Notation "a  '<s='  b" := (Binop (Bits2 (Compare true  cLe _)) (delay_tau a) (delay_tau b)) (in custom koika_t at level 79).
-Notation "a  '>'  b"   := (Binop (Bits2 (Compare false cGt _)) (delay_tau a) (delay_tau b)) (in custom koika_t at level 79).
-Notation "a  '>s'  b"  := (Binop (Bits2 (Compare true  cGt _)) (delay_tau a) (delay_tau b)) (in custom koika_t at level 79).
-Notation "a  '>='  b"  := (Binop (Bits2 (Compare false cGe _)) (delay_tau a) (delay_tau b)) (in custom koika_t at level 79).
-Notation "a  '>s='  b" := (Binop (Bits2 (Compare true  cGe _)) (delay_tau a) (delay_tau b)) (in custom koika_t at level 79).
+Notation "a  '<'  b"   := (delay_tau (Binop (Bits2 (Compare false cLt _)) a b)) (in custom koika_t at level 79).
+Notation "a  '<s'  b"  := (delay_tau (Binop (Bits2 (Compare true  cLt _)) a b)) (in custom koika_t at level 79).
+Notation "a  '<='  b"  := (delay_tau (Binop (Bits2 (Compare false cLe _)) a b)) (in custom koika_t at level 79).
+Notation "a  '<s='  b" := (delay_tau (Binop (Bits2 (Compare true  cLe _)) a b)) (in custom koika_t at level 79).
+Notation "a  '>'  b"   := (delay_tau (Binop (Bits2 (Compare false cGt _)) a b)) (in custom koika_t at level 79).
+Notation "a  '>s'  b"  := (delay_tau (Binop (Bits2 (Compare true  cGt _)) a b)) (in custom koika_t at level 79).
+Notation "a  '>='  b"  := (delay_tau (Binop (Bits2 (Compare false cGe _)) a b)) (in custom koika_t at level 79).
+Notation "a  '>s='  b" := (delay_tau (Binop (Bits2 (Compare true  cGe _)) a b)) (in custom koika_t at level 79).
 
 (* Bit concatenation / shifts *)
-Notation "a  '++'  b"  := (Binop (Bits2 (Concat _ _))          (delay_tau a) (delay_tau b)) (in custom koika_t at level 75).
-Notation "a  '>>'  b"  := (Binop (Bits2 (Lsr _ _))             (delay_tau a) (delay_tau b)) (in custom koika_t at level 74).
-Notation "a  '>>>'  b" := (Binop (Bits2 (Asr _ _))             (delay_tau a) (delay_tau b)) (in custom koika_t at level 74).
-Notation "a  '<<'  b"  := (Binop (Bits2 (Lsl _ _))             (delay_tau a) (delay_tau b)) (in custom koika_t at level 74).
+Notation "a  '++'  b"  := (delay_tau (Binop (Bits2 (Concat _ _))          a b)) (in custom koika_t at level 75).
+Notation "a  '>>'  b"  := (delay_tau (Binop (Bits2 (Lsr _ _))             a b)) (in custom koika_t at level 74).
+Notation "a  '>>>'  b" := (delay_tau (Binop (Bits2 (Asr _ _))             a b)) (in custom koika_t at level 74).
+Notation "a  '<<'  b"  := (delay_tau (Binop (Bits2 (Lsl _ _))             a b)) (in custom koika_t at level 74).
 
 (* Arithmetic *)
-Notation "a  '+'  b"   := (Binop (Bits2 (Plus     _))          (delay_tau a) (delay_tau b)) (in custom koika_t at level 70).
-Notation "a  '-'  b"   := (Binop (Bits2 (Minus    _))          (delay_tau a) (delay_tau b)) (in custom koika_t at level 70).
-Notation "a  '*'  b"   := (Binop (Bits2 (Mul    _ _))          (delay_tau a) (delay_tau b)) (in custom koika_t at level 69).
+Notation "a  '+'  b"   := (delay_tau (Binop (Bits2 (Plus     _))          a b)) (in custom koika_t at level 70).
+Notation "a  '-'  b"   := (delay_tau (Binop (Bits2 (Minus    _))          a b)) (in custom koika_t at level 70).
+Notation "a  '*'  b"   := (delay_tau (Binop (Bits2 (Mul    _ _))          a b)) (in custom koika_t at level 69).
 
 (* Unary operators *)
-Notation "'!' a"       := (Unop  (Bits1 (Not _))               (delay_tau a)) (in custom koika_t at level 65, format "'!' a").
+Notation "'!' a"       := (delay_tau (Unop  (Bits1 (Not _)) a)) (in custom koika_t at level 65, format "'!' a").
 
-Notation "a '[' b ']'"        := (Binop (Bits2 (Sel _))            (delay_tau a) (delay_tau b)) (in custom koika_t at level 60, format "'[' a [ b ] ']'").
-Notation "a '[' b ':+' c ']'" := (Binop (Bits2 (IndexedSlice _ c)) (delay_tau a) (delay_tau b)) (in custom koika_t at level 60, c constr at level 0, format "'[' a [ b :+ c ] ']'").
+Notation "a '[' b ']'"        := (delay_tau (Binop (Bits2 (Sel _))            a b)) (in custom koika_t at level 60, format "'[' a [ b ] ']'").
+Notation "a '[' b ':+' c ']'" := (delay_tau (Binop (Bits2 (IndexedSlice _ c)) a b)) (in custom koika_t at level 60, c constr at level 0, format "'[' a [ b :+ c ] ']'").
 
 
 Class TypeOfSig {sig : Type} (s : sig) := type_of_sig : type.
@@ -294,23 +260,25 @@ Class TypeOfSig {sig : Type} (s : sig) := type_of_sig : type.
 #[export] Instance type_of_array_sig  {s} : @TypeOfSig array_sig  s := array_t s.
 Arguments type_of_sig {sig} s {TypeOfSig} : assert.
 
-Notation "expr : sig" := (Unop (Conv (type_of_sig sig) Unpack) (delay_tau expr))
+Notation "expr : sig" := (delay_tau (Unop (Conv (type_of_sig sig) Unpack) expr))
   (in custom koika_t at level 2, sig constr at level 0).
 
-Notation "expr : 'bits'" := (Unop (Conv _ Pack) (delay_tau expr))
+Notation "expr : 'bits'" := (delay_tau (Unop (Conv _ Pack) expr))
   (in custom koika_t at level 2).
 
-(* for some reason, using struct_idx coq can infer the parameter
-'sig' from the return type, by using StructIdx however, coq fails *)
-(* Definition test : struct_index (Build_struct_sig' type "" [("foo", bits_t 1);("bar", bits_t 5)]) := struct_idx _ "foo". *)
-(* Definition test' : struct_index (Build_struct_sig' type "" [("foo", bits_t 1);("bar", bits_t 5)]) := _ : StructIdx _ "foo". *)
 Class StructIdx sig (f : string) := struct_idx : struct_index sig.
 Hint Mode StructIdx + + : typeclass_instances.
 Arguments struct_idx sig f {StructIdx} : assert.
 Hint Extern 1 (StructIdx ?sig ?f) => exact (must (List_assoc f sig.(struct_fields))) : typeclass_instances.
 
+(* TODO explain why *)
+(* for some reason, using struct_idx coq can infer the parameter
+'sig' from the return type, by using StructIdx however, coq fails *)
+(* Definition test : struct_index (Build_struct_sig' type "" [("foo", bits_t 1);("bar", bits_t 5)]) := struct_idx _ "foo". *)
+(* Definition test' : struct_index (Build_struct_sig' type "" [("foo", bits_t 1);("bar", bits_t 5)]) := _ : StructIdx _ "foo". *)
+
 Notation "v '.[' f ']'" :=
-  (Unop (Struct1 GetField _ (struct_idx _ f)) (delay_tau v))
+  (delay_tau (Unop (Struct1 GetField _ (struct_idx _ f)) v))
   (in custom koika_t at level 0, f custom koika_t_var, format "v .[ f ]").
 
 Notation "'`' a '`'" := (a) (in custom koika_t, a constr).
@@ -339,15 +307,14 @@ Notation "'#' s" := (Const (tau := bits_t _) s) (in custom koika_t at level 0, s
  *   Thus, the same restrictions apply.
  *)
 
-Notation "a" := (Var (var_ref (ident_to_string a) _)) (in custom koika_t at level 0, a constr at level 0, only parsing).
-(* Notation "a" := (Var (mem_eq (var_ref (ident_to_string a) _))) (in custom koika_t at level 0, a constr at level 0, only parsing). *)
-Notation "a" := (Var a) (in custom koika_t at level 0, a constr at level 0, only printing).
+Notation "a" := (delay_tau (Var (var_ref (ident_to_string a) _))) (in custom koika_t at level 0, a constr at level 0, only parsing).
+Notation "a" := (delay_tau (Var (k := a) _)) (in custom koika_t at level 0, a constr at level 0, only printing).
 
 (* Alternative shorter set syntax
  * Note: expr is level 89 to stay below ';' *)
 Export (hints) IdentParsing.TC.
-Notation "a ':=' b" := (let aa := (TC.ident_to_string a) in Assign (var_ref aa _) (delay_tau b)) (in custom koika_t at level 0, a constr at level 0, b custom koika_t at level 89, only parsing).
-Notation "a ':=' b" := (                                    Assign a              (delay_tau b)) (in custom koika_t at level 0, a constr at level 0, b custom koika_t at level 89, only printing).
+Notation "a ':=' b" := (delay_tau (let aa := (TC.ident_to_string a) in Assign (var_ref aa _) b)) (in custom koika_t at level 0, a constr at level 0, b custom koika_t at level 89, only parsing).
+Notation "a ':=' b" := (delay_tau (                                    Assign a              b)) (in custom koika_t at level 0, a constr at level 0, b custom koika_t at level 89, only printing).
 
 (* Koika_args *)
 (* TODO support trailing comma *)
@@ -356,20 +323,19 @@ Notation "'(' x ',' .. ',' y ')'" := (CtxCons (_,_) (x) .. (CtxCons (_,_) (y) Ct
 Notation "'(' ')'" := (CtxEmpty) (in custom koika_t_args).
 Notation "'()'"    := (CtxEmpty) (in custom koika_t_args).
 
-(* TODO generalize delay_tau for a whole argument context *)
 Notation "fn args" :=
-  (InternalCall fn args)
+  (delay_tau (InternalCall fn args))
     (in custom koika_t at level 0, fn constr at level 0, args custom koika_t_args, only parsing).
 
 Notation "instance  '.(' fn ')' args" :=
-  (InternalCall {|
+  (delay_tau (InternalCall {|
     int_name := fn.(int_name);
     int_body := (lift {| lift_fn := instance; lift_comm := eq_refl |}
-                      _ fn.(int_body)) |} args)
+                      _ fn.(int_body)) |} args))
     (in custom koika_t at level 0, instance constr at level 0, fn constr, args custom koika_t_args).
 
 Notation "'{' fn '}' args" :=
-  (InternalCall fn args )
+  (delay_tau (InternalCall fn args))
     (in custom koika_t at level 0, fn constr, args custom koika_t_args, only parsing).
 
 (* ========================================================================= *)
@@ -385,43 +351,60 @@ Notation "'fail'"            := (Fail     unit_t) (in custom koika_t, format "'f
 Notation "'fail' '(' t ')'"  := (Fail (bits_t t)) (in custom koika_t, t constr, format "'fail' '(' t ')'").
 Notation "'fail' '@(' t ')'" := (Fail          t) (in custom koika_t, t constr ,format "'fail' '@(' t ')'").
 
-Notation "'read0' '(' reg ')' "       := (Read P0 reg)                (in custom koika_t, reg constr, format "'read0' '(' reg ')'").
-Notation "'read1' '(' reg ')' "       := (Read P1 reg)                (in custom koika_t, reg constr, format "'read1' '(' reg ')'").
-Notation "'write0' '(' reg ',' v ')'" := (Write P0 reg (delay_tau v)) (in custom koika_t, reg constr, format "'write0' '(' reg ',' v ')'").
-Notation "'write1' '(' reg ',' v ')'" := (Write P1 reg (delay_tau v)) (in custom koika_t, reg constr, format "'write1' '(' reg ',' v ')'").
+Notation "'read0' '(' reg ')' "       := (delay_tau (Read P0 reg)   ) (in custom koika_t, reg constr, format "'read0' '(' reg ')'").
+Notation "'read1' '(' reg ')' "       := (delay_tau (Read P1 reg)   ) (in custom koika_t, reg constr, format "'read1' '(' reg ')'").
+Notation "'write0' '(' reg ',' v ')'" := (delay_tau (Write P0 reg v)) (in custom koika_t, reg constr, format "'write0' '(' reg ',' v ')'").
+Notation "'write1' '(' reg ',' v ')'" := (delay_tau (Write P1 reg v)) (in custom koika_t, reg constr, format "'write1' '(' reg ',' v ')'").
 
-Notation "'zeroExtend(' a ',' b ')'" := (Unop (Bits1 (ZExtL _ b)) (delay_tau a)) (in custom koika_t, b constr, format "'zeroExtend(' a ',' b ')'").
-Notation "'sext(' a ',' b ')'"       := (Unop (Bits1 (SExt  _ b)) (delay_tau a)) (in custom koika_t, b constr, format "'sext(' a ',' b ')'").
+Notation "'zeroExtend(' a ',' b ')'" := (delay_tau (Unop (Bits1 (ZExtL _ b)) a)) (in custom koika_t, b constr, format "'zeroExtend(' a ',' b ')'").
+Notation "'sext(' a ',' b ')'"       := (delay_tau (Unop (Bits1 (SExt  _ b)) a)) (in custom koika_t, b constr, format "'sext(' a ',' b ')'").
 
-Notation "'ignore(' a ')'"       := (Unop (Conv _ Ignore) (delay_tau a)) (in custom koika_t).
-Notation "'pack(' a ')'"         := (Unop (Conv _ Pack)   (delay_tau a)) (in custom koika_t).
-Notation "'unpack(' t ',' v ')'" := (Unop (Conv t Unpack) (delay_tau v)) (in custom koika_t, t constr).
+Notation "'ignore(' a ')'"       := (delay_tau (Unop (Conv _ Ignore) a)) (in custom koika_t).
+Notation "'pack(' a ')'"         := (delay_tau (Unop (Conv _ Pack)   a)) (in custom koika_t).
+Notation "'unpack(' t ',' v ')'" := (delay_tau (Unop (Conv t Unpack) v)) (in custom koika_t, t constr).
 
-Notation "'extcall' method '(' arg ')'" := (ExternalCall method (delay_tau arg)) (in custom koika_t, method constr at level 0).
+Notation "'extcall' method '(' arg ')'" := (delay_tau (ExternalCall method arg)) (in custom koika_t, method constr at level 0).
 
 Notation "'subst' '(' v ',' f ',' a ')'" :=
-  (Binop (Struct2 SubstField _ (struct_idx _ f)) (delay_tau v) (delay_tau a))
-  (in custom koika_t, f custom koika_t_var, format "'subst' '(' v ','  f ',' a ')'").
+  (delay_tau (Binop (Struct2 SubstField _ (struct_idx _ f)) v a))
+  (in custom koika_t, f custom koika_t_var, format "subst ( v ,  f , a )").
 
-Notation "'getbits@' sig '(' v ',' f ')'" :=
-  (Unop  (Bits1 (GetFieldBits   sig (must (List_assoc f sig.(struct_fields))))) (delay_tau v))
-  (in custom koika_t, sig constr at level 0, f custom koika_t_var,
-    format "'getbits@' sig '(' v ','  f ')'").
-Notation "'substbits@' sig '(' v ',' f ',' a ')'" :=
-  (Binop (Bits2 (SubstFieldBits sig (must (List_assoc f sig.(struct_fields))))) (delay_tau v) (delay_tau a))
-  (in custom koika_t, sig constr at level 0, f custom koika_t_var,
-    format "'substbits@' sig '(' v ','  f ','  a ')'").
+Notation "'get' '(' v ',' f ')'" :=
+  (delay_tau (Unop (Struct1 GetField _ (struct_idx _ f)) v))
+  (in custom koika_t, f custom koika_t_var, format "get ( v ,  f )").
+
+Notation "'getbits' '(' t ',' v ',' f ')'" :=
+  (delay_tau (Unop  (Bits1 (GetFieldBits t (struct_idx t f))) v))
+  (in custom koika_t, f custom koika_t_var, t constr, format "getbits ( t ,  v ,  f )").
+
+Notation "'substbits' '(' t ',' v ',' f ',' a ')'" :=
+  (delay_tau (Binop (Bits2 (SubstFieldBits t (struct_idx t f))) v a))
+  (in custom koika_t, f custom koika_t_var, t constr, format "substbits ( t ,  v ,  f ,  a )").
 
 (* TODO evaluate what this array feature should do and how far it is implemented *)
-(* Notation "'aref' '(' v ',' f ')'"                   := (Unop  (Array1  (UGetElement         f)) v)   (in custom koika_t at level 1,                       v custom koika_t at level 13,                             f constr at level 0,           format "'aref' '(' v ','  f ')'").
-Notation "'arefbits' '(' t ',' v ',' f ')'"         := (Unop  (Array1  (UGetElementBits   t f)) v)   (in custom koika_t at level 1, t constr at level 11, v custom koika_t at level 13,                             f constr at level 0,           format "'arefbits' '(' t ','  v ','  f ')'").
-Notation "'asubst' '(' v ',' f ',' a ')'"           := (Binop (Array2  (USubstElement       f)) v a) (in custom koika_t at level 1,                       v custom koika_t at level 13, a custom koika_t at level 13, f constr at level 0,           format "'asubst' '(' v ','  f ',' a ')'").
-Notation "'asubstbits' '(' t ',' v ',' f ',' a ')'" := (Binop (Array2  (USubstElementBits t f)) v a) (in custom koika_t at level 1, t constr at level 11, v custom koika_t at level 13, a custom koika_t at level 13, f constr at level 0,           format "'asubstbits' '(' t ','  v ','  f ',' a ')'").  *)
+(* Notation "'aref' '(' v ',' f ')'"                   := (delay_tau (Unop  (Array1  GetElement sig idx(f) )) v))   (in custom koika_t at level 1,                       v custom koika_t at level 13,                             f constr at level 0,           format "'aref' '(' v ','  f ')'").
+Notation "'arefbits' '(' t ',' v ',' f ')'"         := (delay_tau (Unop  (Array1  (UGetElementBits   t f)) v))   (in custom koika_t at level 1, t constr at level 11, v custom koika_t at level 13,                             f constr at level 0,           format "'arefbits' '(' t ','  v ','  f ')'").
+Notation "'asubst' '(' v ',' f ',' a ')'"           := (delay_tau (Binop (Array2  (USubstElement       f)) v a)) (in custom koika_t at level 1,                       v custom koika_t at level 13, a custom koika_t at level 13, f constr at level 0,           format "'asubst' '(' v ','  f ',' a ')'").
+Notation "'asubstbits' '(' t ',' v ',' f ',' a ')'" := (delay_tau (Binop (Array2  (USubstElementBits t f)) v a)) (in custom koika_t at level 1, t constr at level 11, v custom koika_t at level 13, a custom koika_t at level 13, f constr at level 0,           format "'asubstbits' '(' t ','  v ','  f ',' a ')'").  *)
+
+(* List with bidirectionality hints *)
+Inductive list' {A : Type} : Type :=
+  | nil'
+  | cons' (a : A) (l : list').
+Arguments list' A : clear implicits.
+Arguments nil' & {A}.
+Arguments cons' & {A} a l.
+
+Inductive prod' {A B : Type} : Type :=
+  | pair' : A → B → prod'.
+Arguments prod' A B : clear implicits.
+Arguments pair' & {A B} _ _.
 
 (* Koika_branches *)
 Declare Custom Entry koika_t_branches.
-Notation "x '=>' a"      := [(x,a)]        (in custom koika_t_branches at level 0, x custom koika_t at level 200, a custom koika_t at level 200).
-Notation "arg1 '|' arg2" := (arg1 ++ arg2) (in custom koika_t_branches at level 1, format "'[v' arg1 ']' '/' '|'  '[v' arg2 ']'").
+Notation "x '=>' a"      := (cons' (pair' x a) nil') (in custom koika_t_branches at level 0, x custom koika_t at level 200, a custom koika_t at level 200).
+Notation "x '=>' a '|' arg2" := (cons' (pair' x a) arg2) (in custom koika_t_branches at level 0, x custom koika_t at level 200, a custom koika_t at level 200).
+(* format "'[v' arg1 ']' '/' '|'  '[v' arg2 ']'" *)
 
 (* TODO total match -> maybe for enums? *)
 (* For example if var has enum type then allow special match with
@@ -434,20 +417,21 @@ thats possible -- but should that be legal?
 *)
 (* TODO move to macros *)
 
+
 Fixpoint macro_switch
   {reg_t ext_fn_t} {R: reg_t -> type} {Sigma: ext_fn_t -> ExternalSignature}
   {sig tau tau_arg}
   (var: action' (tau := tau_arg) R Sigma)
   (default: action' (tau := tau) R Sigma)
-  (branches: list (action' (tau := tau_arg) R Sigma * action' (tau := tau) (sig := sig) R Sigma))
+  (branches: list' (prod' (action' (tau := tau_arg) R Sigma) (action' (tau := tau) (sig := sig) R Sigma)))
     : action' (tau := tau) (sig := sig) R Sigma :=
   match branches with
-  | nil => default
-  | (label, act) :: branches =>
+  | nil' => default
+  | cons' (pair' label act) branches =>
     If (Binop (Eq _ false) var label) act (macro_switch var default branches)
   end.
 Notation "'match' var 'with' '|' branches 'return' 'default' ':' default 'end'" :=
-  (macro_switch var default branches)
+  (delay_tau (macro_switch var default branches))
     (in custom koika_t, branches custom koika_t_branches,
       format "match  var  with '/' '[v'  |  branches '/' return  default :  default ']' end").
 
@@ -468,18 +452,16 @@ Notation "'Ob'" := (Const (tau := unit_t) Ob)
   (in custom koika_t at level 0, format "'Ob'").
 
 (* koika bit vector literals *)
+Class Default {A} (a:A) := default : A.
+Arguments default {A} a {Default}.
+(* TODO: I am hoping that this low priority makes sure that the resolution of Default
+  only happens after all other type classes have been resolved - however, I currently have
+  no clue if it even has an influence on the resolution order of different classes *)
+Hint Extern 9999 (Default ?a) => exact (a) : typeclass_instances.
 
-Local Definition len := String.length.
+Definition test_default1 : bits _ := Bits.of_N (default 10) 0.
+Definition test_default2 : bits 5 := Bits.of_N (default 10) 0.
 
-(* Bits.of_N with an inferred length or a default if inference fails *)
-Ltac bits_of_N default val :=
-  exact (Bits.of_N default val) + exact (Bits.of_N _ val).
-  (* match goal with
-  | |- bits ?n =>
-    tryif has_evar n
-    then exact (Bits.of_N default val)
-    else exact (Bits.of_N _ val)
-  end. *)
 (* TODO maybe parse numbers like this *)
 (* Check (ident_to_string Ob001100). *)
 
@@ -531,31 +513,33 @@ Ltac bits_of_N default val :=
  * instead of a '0' to let coq parse them as an ident instead of a number, e.g.
  * Ox9C0FFE is a totally valid ident for coq)
  *)
-Notation "num ':b' sz" := (Const (tau := bits_t  _)      (Bits.of_N (sz <: nat)            (bin_string_to_N num))) (in custom koika_t at level 0, num constr at level 0, sz constr at level 0, only parsing).
-Notation "num ':b'"    := (Const (tau := bits_t  _) ltac:(bits_of_N ((len num) * 1)        (bin_string_to_N num))) (in custom koika_t at level 0, num constr at level 0,                       only parsing).
-Notation "'0b' num sz" := (Const (tau := bits_t sz)      (Bits.of_N (sz <: nat)            (bin_string_to_N num))) (in custom koika_t at level 0, num constr at level 0, sz constr at level 0, format "'0b' num sz").
-Notation "'0b' num"    := (Const (tau := bits_t  _) ltac:(bits_of_N ((len num) * 1)        (bin_string_to_N num))) (in custom koika_t at level 0, num constr at level 0,                       only parsing).
-Notation "'0b' num"    := (Const (tau := bits_t  _)      (Bits.of_N _                      (bin_string_to_N num))) (in custom koika_t at level 0, num constr at level 0, only printing,        format "'0b' num").
+Local Definition len := String.length.
 
-Notation "num ':o' sz" := (Const (tau := bits_t _)      (Bits.of_N (sz <: nat)            (oct_string_to_N num))) (in custom koika_t at level 0, num constr at level 0, sz constr at level 0, only parsing).
-Notation "num ':o'"    := (Const (tau := bits_t _) ltac:(bits_of_N ((len num) * 3)        (oct_string_to_N num))) (in custom koika_t at level 0, num constr at level 0,                       only parsing).
-Notation "'0o' num sz" := (Const (tau := bits_t _)      (Bits.of_N (sz <: nat)            (oct_string_to_N num))) (in custom koika_t at level 0, num constr at level 0, sz constr at level 0, format "'0o' num sz").
-Notation "'0o' num"    := (Const (tau := bits_t _) ltac:(bits_of_N ((len num) * 3)        (oct_string_to_N num))) (in custom koika_t at level 0, num constr at level 0,                       only parsing).
-Notation "'0o' num"    := (Const (tau := bits_t _)      (Bits.of_N _                      (oct_string_to_N num))) (in custom koika_t at level 0, num constr at level 0, only printing,        format "'0o' num").
+Notation "num ':b' sz" := (Const (tau := bits_t  _) (Bits.of_N (sz <: nat)                    (bin_string_to_N num))) (in custom koika_t at level 0, num constr at level 0, sz constr at level 0, only parsing).
+Notation "num ':b'"    := (Const (tau := bits_t  _) (Bits.of_N (default ((len num) * 1))      (bin_string_to_N num))) (in custom koika_t at level 0, num constr at level 0,                       only parsing).
+Notation "'0b' num sz" := (Const (tau := bits_t sz) (Bits.of_N (sz <: nat)                    (bin_string_to_N num))) (in custom koika_t at level 0, num constr at level 0, sz constr at level 0, format "'0b' num sz").
+Notation "'0b' num"    := (Const (tau := bits_t  _) (Bits.of_N (default ((len num) * 1))      (bin_string_to_N num))) (in custom koika_t at level 0, num constr at level 0,                       only parsing).
+Notation "'0b' num"    := (Const (tau := bits_t  _) (Bits.of_N _                              (bin_string_to_N num))) (in custom koika_t at level 0, num constr at level 0, only printing,        format "'0b' num").
 
-Notation "num ':d' sz" := (Const (tau := bits_t _)      (Bits.of_N (sz <: nat)            (dec_string_to_N num))) (in custom koika_t at level 0, num constr at level 0, sz constr at level 0, only parsing).
-Notation "num ':d'"    := (Const (tau := bits_t _) ltac:(bits_of_N (1 + (N.to_nat (N.log2 (dec_string_to_N num))))
-                                                                                          (dec_string_to_N num))) (in custom koika_t at level 0, num constr at level 0,                       only parsing).
-Notation "'0d' num sz" := (Const (tau := bits_t _)      (Bits.of_N (sz <: nat)            (dec_string_to_N num))) (in custom koika_t at level 0, num constr at level 0, sz constr at level 0, format "'0d' num sz").
-Notation "'0d' num"    := (Const (tau := bits_t _) ltac:(bits_of_N (1 + (N.to_nat (N.log2 (dec_string_to_N num))))
-                                                                                          (dec_string_to_N num))) (in custom koika_t at level 0, num constr at level 0,                       only parsing).
-Notation "'0d' num"    := (Const (tau := bits_t _)      (Bits.of_N _                      (dec_string_to_N num))) (in custom koika_t at level 0, num constr at level 0, only printing,        format "'0d' num").
+Notation "num ':o' sz" := (Const (tau := bits_t _) (Bits.of_N (sz <: nat)                     (oct_string_to_N num))) (in custom koika_t at level 0, num constr at level 0, sz constr at level 0, only parsing).
+Notation "num ':o'"    := (Const (tau := bits_t _) (Bits.of_N (default ((len num) * 3))       (oct_string_to_N num))) (in custom koika_t at level 0, num constr at level 0,                       only parsing).
+Notation "'0o' num sz" := (Const (tau := bits_t _) (Bits.of_N (sz <: nat)                     (oct_string_to_N num))) (in custom koika_t at level 0, num constr at level 0, sz constr at level 0, format "'0o' num sz").
+Notation "'0o' num"    := (Const (tau := bits_t _) (Bits.of_N (default ((len num) * 3))       (oct_string_to_N num))) (in custom koika_t at level 0, num constr at level 0,                       only parsing).
+Notation "'0o' num"    := (Const (tau := bits_t _) (Bits.of_N _                               (oct_string_to_N num))) (in custom koika_t at level 0, num constr at level 0, only printing,        format "'0o' num").
 
-Notation "num ':h' sz" := (Const (tau := bits_t _)      (Bits.of_N (sz <: nat)            (hex_string_to_N num))) (in custom koika_t at level 0, num constr at level 0, sz constr at level 0, only parsing).
-Notation "num ':h'"    := (Const (tau := bits_t _) ltac:(bits_of_N ((len num) * 4)        (hex_string_to_N num))) (in custom koika_t at level 0, num constr at level 0,                       only parsing).
-Notation "'0x' num sz" := (Const (tau := bits_t _)      (Bits.of_N (sz <: nat)            (hex_string_to_N num))) (in custom koika_t at level 0, num constr at level 0, sz constr at level 0, format "'0x' num sz").
-Notation "'0x' num"    := (Const (tau := bits_t _) ltac:(bits_of_N ((len num) * 4)        (hex_string_to_N num))) (in custom koika_t at level 0, num constr at level 0,                       only parsing).
-Notation "'0x' num"    := (Const (tau := bits_t _)      (Bits.of_N _                      (hex_string_to_N num))) (in custom koika_t at level 0, num constr at level 0, only printing,        format "'0x' num").
+Notation "num ':d' sz" := (Const (tau := bits_t _) (Bits.of_N (sz <: nat)                     (dec_string_to_N num))) (in custom koika_t at level 0, num constr at level 0, sz constr at level 0, only parsing).
+Notation "num ':d'"    := (Const (tau := bits_t _) (Bits.of_N (default (1 + (N.to_nat (N.log2 (dec_string_to_N num)))))
+                                                                                              (dec_string_to_N num))) (in custom koika_t at level 0, num constr at level 0,                       only parsing).
+Notation "'0d' num sz" := (Const (tau := bits_t _) (Bits.of_N (sz <: nat)                     (dec_string_to_N num))) (in custom koika_t at level 0, num constr at level 0, sz constr at level 0, format "'0d' num sz").
+Notation "'0d' num"    := (Const (tau := bits_t _) (Bits.of_N (default (1 + (N.to_nat (N.log2 (dec_string_to_N num)))))
+                                                                                              (dec_string_to_N num))) (in custom koika_t at level 0, num constr at level 0,                       only parsing).
+Notation "'0d' num"    := (Const (tau := bits_t _) (Bits.of_N _                               (dec_string_to_N num))) (in custom koika_t at level 0, num constr at level 0, only printing,        format "'0d' num").
+
+Notation "num ':h' sz" := (Const (tau := bits_t _) (Bits.of_N (sz <: nat)                     (hex_string_to_N num))) (in custom koika_t at level 0, num constr at level 0, sz constr at level 0, only parsing).
+Notation "num ':h'"    := (Const (tau := bits_t _) (Bits.of_N (default ((len num) * 4))       (hex_string_to_N num))) (in custom koika_t at level 0, num constr at level 0,                       only parsing).
+Notation "'0x' num sz" := (Const (tau := bits_t _) (Bits.of_N (sz <: nat)                     (hex_string_to_N num))) (in custom koika_t at level 0, num constr at level 0, sz constr at level 0, format "'0x' num sz").
+Notation "'0x' num"    := (Const (tau := bits_t _) (Bits.of_N (default ((len num) * 4))       (hex_string_to_N num))) (in custom koika_t at level 0, num constr at level 0,                       only parsing).
+Notation "'0x' num"    := (Const (tau := bits_t _) (Bits.of_N _                               (hex_string_to_N num))) (in custom koika_t at level 0, num constr at level 0, only printing,        format "'0x' num").
 
 (* legacy number format *)
 Notation "'|' a '`d' b '|'" := (Const (tau := bits_t _) (Bits.of_N (a<:nat) b%N)) (in custom koika_t at level 0, a constr at level 0, b constr at level 0).
@@ -571,18 +555,21 @@ Section Macro.
 
   (* A koika action which build a struct instance filled
   with zeroes *)
-  Definition struct_init_zeros {sig} (tau: type) : action' (sig := sig) R Sigma :=
-    Unop (Conv tau Unpack) (Const (tau := bits_t _) (Bits.zeroes (type_sz tau))).
+  Definition const_zero {sig} (tau: type) : action' (tau := tau) (sig := sig) R Sigma :=
+    Const (value_of_bits (Bits.zero)).
 
+  Inductive sigT' {A: Type} (P: A -> Type) : Type :=
+    existT' : forall x:A, P x -> sigT' P.
+  Arguments existT' & {A} P _ _.
   (* Transforming a list of actions into a sequence of
   substitute operations to initialize a struct *)
   Fixpoint struct_init {sig} (s_sig: struct_sig)
-    (fields: list {idx : struct_index s_sig & (action' (tau := field_type s_sig idx) (sig := sig) R Sigma)})
+    (fields: list' (sigT' (A := struct_index s_sig) (fun idx => (action' (tau := field_type s_sig idx) (sig := sig) R Sigma))))
     : action' (sig := sig) R Sigma :=
     match fields with
-    | (idx;act) :: fields' =>
+    | cons' (existT' _ idx act) fields' =>
       (Binop (Struct2 SubstField s_sig idx)) (struct_init s_sig fields') act
-    | [] => struct_init_zeros (struct_t s_sig)
+    | nil' => const_zero (struct_t s_sig)
     end.
 
   (* The struct's signature needs to be known to check if a given field exists within
@@ -592,37 +579,36 @@ Section Macro.
   makes sure that the index computation is deferred and only executed after the signature
   is known *)
   Class FieldSubst {tau sig} (s_sig : struct_sig) (field : string) (a : action' (sig := sig) (tau := tau) R Sigma) :=
-    field_subst : {idx : struct_index s_sig & (action' (sig := sig) (tau := field_type s_sig idx) R Sigma )}.
-
+    field_subst : (sigT' (A := struct_index s_sig) (fun idx => (action' (sig := sig) (tau := field_type s_sig idx) R Sigma))).
 End Macro.
-Hint Mode FieldSubst + + + + + + + + + : typeclass_instances.
-Arguments field_subst {reg_t ext_fn_t} {R Sigma} {tau sig} s_sig field a {FieldSubst} : assert.
-Hint Extern 1 (FieldSubst ?sig ?field ?a) => exact ((must (List_assoc field sig.(struct_fields)) ; a)) : typeclass_instances.
 
+Hint Mode FieldSubst + + + + + + + + + : typeclass_instances.
+Arguments field_subst & {reg_t ext_fn_t} {R Sigma} {tau sig} s_sig field a {FieldSubst} : assert.
+Hint Extern 1 (FieldSubst ?sig ?field ?a) => exact (existT' _ (must (List_assoc field sig.(struct_fields))) a) : typeclass_instances.
 Declare Custom Entry koika_t_struct.
 Declare Custom Entry koika_t_struct_field.
+
 (* struct instantiation in koika *)
 (* expr at level at level 89 to stay below koika's sequence (a ; b) *)
 Notation "f ':=' expr" := (field_subst _ f expr)
   (in custom koika_t_struct_field at level 0, f custom koika_t_var, expr custom koika_t at level 89).
-Notation "a ';' b" := (cons a b)   (in custom koika_t_struct at level 0, a custom koika_t_struct_field, right associativity).
-Notation "a ';'"   := (cons a nil) (in custom koika_t_struct at level 0, a custom koika_t_struct_field). (* trailing comma *)
-Notation "a"       := (cons a nil) (in custom koika_t_struct at level 0, a custom koika_t_struct_field).
-
+Notation "a ';' b" := (cons' a b)   (in custom koika_t_struct at level 0, a custom koika_t_struct_field, right associativity).
+Notation "a ';'"   := (cons' a nil') (in custom koika_t_struct at level 0, a custom koika_t_struct_field). (* trailing comma *)
+Notation "a"       := (cons' a nil') (in custom koika_t_struct at level 0, a custom koika_t_struct_field).
 
 Notation "'struct' sig '::{' '}'" :=
-  (struct_init sig []) (in custom koika_t, sig constr at level 0).
+  (delay_tau (const_zero (struct_t sig))) (in custom koika_t, sig constr at level 0).
 
 Notation "'struct' sig '::{' fields '}'" :=
-  (struct_init sig fields) (in custom koika_t, sig constr at level 0,
+  (delay_tau (struct_init sig fields)) (in custom koika_t, sig constr at level 0,
   fields custom koika_t_struct).
 
 (* Needs the same level as 'Var' + level of first non-terminal must match *)
 Notation "sig '::{' '}'" :=
-  (struct_init sig []) (in custom koika_t at level 0, sig constr at level 0).
+  (delay_tau (const_zero (struct_t sig))) (in custom koika_t at level 0, sig constr at level 0).
 
 Notation "sig '::{' fields '}'" :=
-  (struct_init sig fields) (in custom koika_t at level 0, sig constr at level 0,
+  (delay_tau (struct_init sig fields)) (in custom koika_t at level 0, sig constr at level 0,
   fields custom koika_t_struct).
 
 Notation "'enum' sig '::<' f '>'" :=
@@ -667,23 +653,7 @@ End TODO_contrs_arg_lists.
  * the outer terms into the inner terms and then they are used to infer the
  * type of registers and variables.                                          *)
 
-Module BidirectionalityHintsTest.
-Section BidirectionalityHintsTest.
-  Inductive reg_t := reg1 | reg2.
-  Definition R (r : reg_t) := match r with
-    | reg1 => bits_t 1
-    | reg2 => bits_t 2
-    end.
-  Context {ext_fn_t : Type}.
-  Context {Sigma: ext_fn_t -> ExternalSignature}.
 
-  Arguments Fail {pos_t var_t fn_name_t reg_t ext_fn_t} {R Sigma} {sig} & tau : assert.
-  Definition test_Fail1 := (Fail (bits_t 3)) : action R Sigma.
-  Definition test_Fail2 := (Fail (_)) : action R Sigma (tau := bits_t 3).
-
-  (* Definition test_write := (Write P0 reg1 (Const Ob~1)) : action R Sigma. *)
-End BidirectionalityHintsTest.
-End BidirectionalityHintsTest.
 
 (* Bidirectionality Hints
  *
@@ -716,24 +686,26 @@ End BidirectionalityHintsTest.
  *)
 
 
-(* Nothing needs to be inferred from the context  *)
-Arguments Fail         {pos_t var_t fn_name_t reg_t ext_fn_t}   {R Sigma} {sig} tau : assert.
-Arguments Var          {pos_t var_t fn_name_t reg_t ext_fn_t} & {R Sigma} {sig} {k tau} m : assert.
-Arguments Const        {pos_t var_t fn_name_t reg_t ext_fn_t}   {R Sigma} {sig tau} cst : assert.
-Arguments Assign       {pos_t var_t fn_name_t reg_t ext_fn_t} & {R Sigma} {sig} {k tau} m ex : assert.
-Arguments Seq          {pos_t var_t fn_name_t reg_t ext_fn_t} & {R Sigma} {sig tau} r1 r2 : assert.
-Arguments Bind         {pos_t var_t fn_name_t reg_t ext_fn_t} & {R Sigma} {sig tau} {tau'} var ex body : assert.
-Arguments If           {pos_t var_t fn_name_t reg_t ext_fn_t} & {R Sigma} {sig tau} cond tbranch fbranch : assert.
-Arguments Read         {pos_t var_t fn_name_t reg_t ext_fn_t} & {R Sigma} {sig} port idx : assert.
-Arguments Write        {pos_t var_t fn_name_t reg_t ext_fn_t} & {R Sigma} {sig} port idx value : assert.
-Arguments Unop         {pos_t var_t fn_name_t reg_t ext_fn_t} & {R Sigma} {sig} fn arg1 : assert.
-Arguments Binop        {pos_t var_t fn_name_t reg_t ext_fn_t} & {R Sigma} {sig} fn arg1 arg2 : assert.
-Arguments ExternalCall {pos_t var_t fn_name_t reg_t ext_fn_t} & {R Sigma} {sig} fn arg : assert.
-Arguments InternalCall {pos_t var_t fn_name_t reg_t ext_fn_t} & {R Sigma} {sig tau} {argspec} fn args : assert.
-(* Arguments APos         {pos_t var_t fn_name_t reg_t ext_fn_t} & {R Sigma} {sig tau} pos a : assert. *)
-Arguments Build_InternalFunction' {fn_name_t action} & int_name int_body : assert.
-Arguments macro_switch {reg_t ext_fn_t} & {R Sigma} {sig} {tau tau_arg} var default branches : assert.
-Arguments struct_init  {reg_t ext_fn_t} & {R Sigma} {sig} s_sig fields : assert.
+(* Nothing needs to be inferred from the context *)
+(* Actions which do neither contain nested actions nor rely on the values of sig, R, or Sigma
+  do not get a hint and are not wrapped in delay_tau in the notations *)
+Arguments Fail           {pos_t var_t fn_name_t reg_t ext_fn_t} {R Sigma} {sig} tau : assert. (* No hint *)
+Arguments Var          & {pos_t var_t fn_name_t reg_t ext_fn_t} {R Sigma} {sig} {k tau} m : assert.
+Arguments Const          {pos_t var_t fn_name_t reg_t ext_fn_t} {R Sigma} {sig tau} cst : assert. (* No hint *)
+Arguments Assign       & {pos_t var_t fn_name_t reg_t ext_fn_t} {R Sigma} {sig} {k tau} m ex : assert.
+Arguments Seq          & {pos_t var_t fn_name_t reg_t ext_fn_t} {R Sigma} {sig tau} r1 r2 : assert.
+Arguments Bind         & {pos_t var_t fn_name_t reg_t ext_fn_t} {R Sigma} {sig tau} {tau'} var ex body : assert.
+Arguments If           & {pos_t var_t fn_name_t reg_t ext_fn_t} {R Sigma} {sig tau} cond tbranch fbranch : assert.
+Arguments Read         & {pos_t var_t fn_name_t reg_t ext_fn_t} {R Sigma} {sig} port idx : assert.
+Arguments Write        & {pos_t var_t fn_name_t reg_t ext_fn_t} {R Sigma} {sig} port idx value : assert.
+Arguments Unop         & {pos_t var_t fn_name_t reg_t ext_fn_t} {R Sigma} {sig} fn arg1 : assert.
+Arguments Binop        & {pos_t var_t fn_name_t reg_t ext_fn_t} {R Sigma} {sig} fn arg1 arg2 : assert.
+Arguments ExternalCall & {pos_t var_t fn_name_t reg_t ext_fn_t} {R Sigma} {sig} fn arg : assert.
+Arguments InternalCall & {pos_t var_t fn_name_t reg_t ext_fn_t} {R Sigma} {sig tau} {argspec} fn args : assert.
+Arguments APos         & {pos_t var_t fn_name_t reg_t ext_fn_t} {R Sigma} {sig tau} pos a : assert. (* that action doesn't even have a notation *)
+Arguments Build_InternalFunction' & {fn_name_t action} int_name int_body : assert.
+Arguments macro_switch & {reg_t ext_fn_t} {R Sigma} {sig} {tau tau_arg} var default branches : assert.
+Arguments struct_init  & {reg_t ext_fn_t} {R Sigma} {sig} s_sig fields : assert.
 
 (* TODO: what does this? *)
 (* Set Typeclasses Dependency Order. *)
@@ -751,8 +723,7 @@ Section Tests'.
   | reg2
   | reg3.
 
-  Definition R (r : reg_t) := bits_t 64.
-  Definition R' (r : reg_t) :=
+  Definition R (r : reg_t) :=
     match r with
     | reg0 => bits_t 64
     | reg1 => bits_t 64
@@ -763,34 +734,27 @@ Section Tests'.
   Context {ext_fn_t : Type}.
   Context {Sigma : ext_fn_t -> ExternalSignature}.
 
-  Definition test_concatenation2 : action' R' Sigma (sig := [("yo", bits_t 4)]) := <{
-    write0(reg2, Ob~1 ++ read0(reg3));
+  Definition test_concatenation : action' R Sigma (sig := [("yo", bits_t 4)]) := <{
+    write0(reg2, Ob~1 ++ read0(reg3))
   }>.
 
-  (* Definition idk5 : @TypedSyntax.action unit string string _ _ R Sigma [("a", R' reg3)] (bits_t 4) := (@Var _ _ _ _ _ _ _ [("a", R' reg3)] "a" (_) (must_class (assoc "a" _)).2). *)
-
-  Arguments Var {pos_t var_t fn_name_t reg_t ext_fn_t} {R Sigma} {sig} & {k tau} m : assert.
-
-  Definition idk6 : @TypedSyntax.action unit string string _ _ R Sigma [("a", R' reg3)] (bits_t 4) := delay_tau (Var (var_ref "a" _)).
-
-  Definition read_reg : action' R' Sigma (sig := [("a", R' reg3)]) (tau := bits_t 4) := <{
+  Definition read_reg : action' R Sigma (sig := [("a", R reg3)]) (tau := bits_t 4) := <{
     a
   }>.
-  Definition read_reg2 : function R' Sigma := <{
+  Definition read_reg2 : function R Sigma := <{
   fun read_reg () : bits_t 4 =>
     let a := if 0b"0" then read0(reg3) else 0b"1010" in
     a
   }>.
-  Definition read_reg3 : (* action' R Sigma (sig:= [("select", bits_t 1)]) (tau := bits_t 64) *) function R Sigma := <{
+  Definition read_reg3 : function R Sigma := <{
   fun read_reg (select : bits_t 1) : bits_t 64 =>
-    let data :=
-      if `tau_eq <{select}>`
+    let data := if select
       then read0(reg1)
       else read0(reg0)
     in data
   }>.
 
-  Definition read_reg' : function R' Sigma := <{
+  Definition read_reg' : function R Sigma := <{
   fun read_reg' (select : bits_t 1) : bits_t 64 =>
     if select
       then read0(reg1)
@@ -902,21 +866,21 @@ Module Type Tests.
   Definition test_cast1 : action R Sigma (tau := enum_t numbers_e) := <{
     0b"001" : numbers_e
   }>.
-  (* Definition test_cast2 : action R Sigma (tau := bits_t 3) := <{ *)
-    (* numbers_e::<ONE> : bits *)
-  (* }>. *)
-  Definition test_cast3 : action R Sigma (tau := struct_t numbers_s) := <{
+  Definition test_cast2 : action R Sigma (tau := bits_t 3) := <{
+    numbers_e::<ONE> : bits
+  }>.
+  Definition test_cast3 : action R Sigma := <{
     0b"001010011" : numbers_s
   }>.
-  (* Definition test_cast4 : action R Sigma (tau := bits_t 9) := <{ *)
-    (* numbers_s::{ } : bits *)
-  (* }>. *)
+  Definition test_cast4 : action R Sigma (tau := bits_t 9) := <{
+    numbers_s::{ } : bits
+  }>.
   Definition test_cast5 : action R Sigma (tau := array_t some_arr) := <{
     0b"1001001101" : some_arr
   }>.
-  (* Definition test_cast6 : action R Sigma (tau := bits_t 10) := <{ *)
-    (* 0b"1001001101" : some_arr : bits *)
-  (* }>. *)
+  Definition test_cast6 : action R Sigma (tau := bits_t 10) := <{
+    0b"1001001101" : some_arr : bits
+  }>.
 End Tests.
 Module Type Tests2.
   Inductive reg_t :=
@@ -962,13 +926,21 @@ Module Type Tests2.
       if a < b then a else b
     }>.
 
-  (* Definition test_select : function R Sigma := <{ *)
-    (* fun sel (v : bits_t 4) : bits_t 2 => *)
-      (* v[0b"01"] ++ v[0b"11"] *)
-  (* }>. *)
+  (* double binders *)
+  Definition min' {reg_t ext_fn_t : Type} {R : reg_t -> type}
+    {Sigma : ext_fn_t -> ExternalSignature}
+    (sz : nat) : function R Sigma := <{
+    fun min (a b: bits_t sz) : bits_t sz =>
+      if a < b then a else b
+    }>.
+
+  Definition test_select : function R Sigma := <{
+    fun sel (v : bits_t 4) : bits_t 2 =>
+      v[0b"01"] ++ v[0b"11"]
+  }>.
 
   Definition idk : _action := <{
-    (read0(data0))[Ob~1~1~1 :+ 3]
+    read0(data0)[Ob~1~1~1 :+ 3]
   }>.
 
   Definition idk2 : _action := <{
@@ -979,7 +951,7 @@ Module Type Tests2.
       ) else pass);
     fail
   }>.
-  (* Definition test_27 : _action := <{
+  Definition test_27 : _action := <{
     ignore(if (!read0(data0))[#(Bits.of_nat _ 0) :+ 1] then (
       write0(data0, 0b"01101");
       let yo := if (Ob~1) then 0b"1001" else 0x"F" in
@@ -987,7 +959,7 @@ Module Type Tests2.
       0b"00011"5
       ) else read0(data0));
     fail
-  }>. *)
+  }>.
   Definition test_28 : _action := <{
     let var := 0b"101" in
     match var with
@@ -1022,31 +994,18 @@ Module Type Tests2.
       ("two"  , bits_t 3) ]
   |}.
 
-  (* Definition get
-  {reg_t ext_fn_t}
-  {R : reg_t -> type}
-  {Sigma : ext_fn_t -> ExternalSignature}
-  {sig ssig}
-  (v : @action' (struct_t ssig) sig _ _ R Sigma)
-  (f : var_t)
-  {si : StructIdx ssig f}
-  : @action' (field_type ssig (struct_idx ssig f)) sig _ _ R Sigma :=
-  (Unop (Struct1 GetField ssig (struct_idx ssig f)) v).
-
-  Arguments get {reg_t ext_fn_t} {R Sigma} {sig ssig} v f & {si} : assert. *)
-Notation "'get' '(' v ',' f ')'" :=
-  (* (get v f) *)
-  (tau_eq (Unop  (Struct1 GetField   _ (struct_idx _ f)) v))
-  (in custom koika_t, f custom koika_t_var, format "'get' '(' v ','  f ')'").
+  Notation "'get' '(' v ',' f ')'" :=
+    (delay_tau (Unop (Struct1 GetField _ (struct_idx _ f)) v))
+    (in custom koika_t, f custom koika_t_var, format "'get' '(' v ','  f ')'").
 
   Definition test_get : function R Sigma := <{
     fun idk (num : struct_t some_s) : bits_t 3 =>
       get(num, one)
   }>.
-  (* Definition test_get : function R Sigma := <{ *)
-    (* fun idk (num : struct_t some_s) : bits_t 10 => *)
-     (* zeroExtend(num.[one], 10) *)
-  (* }>. *)
+  Definition test_get2 : function R Sigma := <{
+    fun idk (num : struct_t some_s) : bits_t 10 =>
+     zeroExtend(num.[one], 10)
+  }>.
 
   Definition test_subst : function R Sigma := <{
     fun idk (num : struct_t some_s) : struct_t some_s =>
